\documentclass{article}
\usepackage{../m}

\begin{document}
\noindent Paul Gustafson\\
\noindent Math 643 - Algebraic Topology I

%Problems: 5.1 (be sure to go through this exercise), 5.2, 5.3*, 5.4, 5.5(ii)* use part (i), 5.7, 5.8, 5.9, 5.10, 5.11* 

\subsection*{HW 7}
\p{5.3} Let 
$$0  \to A \overset i \to B \overset p \to C \to 0$$
be a short exact sequence. Show that $iA \simeq A$ and $B/iA \simeq C$.
\begin{proof}
The kernel of $i$ is trivial so the map is a bijection onto $iA$, hence an isomorphism $A \to iA$.

The kernel of $B \to C$ is $iA$ and $B \to C$ is surjective, hence the induced map $B/iA \to C$ is an isomorphism.
\end{proof}

\p{5.5(ii)} If $0 \to A_n \to A_{n-1} \to \ldots \to A_1 \to A_0 \to 0$ is an exact sequence of f.g. abelian groups, then
$\sum_{i=0}^n (-1)^i \rank A_i = 0$.
\begin{proof}
We use strong induction on $n$. Part (i) covers the cases $n \le 2$. For $n > 3$, pick $j$ to be greatest integer at most $n/2$.
Then $0 \to A_n \to \ldots to A_j \to B \to 0$ and $0 \to B \to A_{j-1} \to \ldots A_0 \to 0$ are exact sequences of shorter length than the original,
where $B$ is the image of the map $A_j \to A_{j-1}$.  By the induction hypothesis, 
$$0 = (-1)^j \rank B + \sum_{i=0}^{j-1} (-1)^i \rank A_i = \rank B + \sum_{i=j}^{n} (-1)^{i-j+1} \rank A_i.$$
By multiplying the last expression by $(-1)^{j-1}$ and adding it to the other, we get the desired equality.
\end{proof}

\p{5.11} If $U_* \subset T_* \subset S_*$ then
$$0 \to T_*/U_*  \overset{i}{\to} S_*/U_* \overset{p}{\to} S_*/T_* \to 0,$$
where $i_n: t_n + U_n \mapsto t_n + U_n$ and $p_n(s_n + U_n) = s_n + T_n$.
\begin{proof}
By the third isomorphism theorem for groups, we get short exact sequences
$$T_n/U_n \overset{i_n}{\to} S_n/U_n \overset{p_n}{\to} S_n/T_n,$$
for every $n$.

Moreover $U_* \subset T_* \subset S_*$ implies that $i$ and $p$ are chain maps,
so we get the desired short exact sequence of chain complexes.
\end{proof}
\end{document}
